proof/theories/Dnat_Rewrite.v
@@ -487,7 +487,7 @@ Definition env0 : env :=
   {| e_set := fun _ => []; e_vmap := fun _ => []; e_map := fun _ => [];
      e_routes := []; e_rt := fun _ => []; e_limit := fun _ => 0;
      e_quota := fun _ => 0; e_ifaddr := fun _ => []; e_ifaddr6 := fun _ => [];
-     e_connlimit := fun _ => 0;
+     e_connlimit := fun _ => [];
      e_ct := fun _ _ => []; e_nat := fun _ => None; e_numgen := fun _ => 0 |}.
 Definition pkt4 : packet :=
   {| pkt_env := env0; pkt_meta := fun _ => []; pkt_ct := fun _ => [];
