proof/theories/Red_LimitProbe.v
@@ -43,7 +43,7 @@ Definition env1 : env :=
      e_routes := []; e_rt := fun _ => [];
      e_limit := fun _ => 1;                 (* exactly one token *)
      e_quota := fun _ => 0; e_ifaddr := fun _ => []; e_ifaddr6 := fun _ => [];
-     e_connlimit := fun _ => 0; e_ct := fun _ _ => []; e_nat := fun _ => None;
+     e_connlimit := fun _ => []; e_ct := fun _ _ => []; e_nat := fun _ => None;
      e_numgen := fun _ => 0 |}.
 
 Definition mkpkt (e : env) (flow : data) : packet :=
